src/computational_monads/simulation_semantics/constructions/logging_oracle.lean
@@ -14,22 +14,54 @@ The implementation is as a `tracking_oracle`, using a `query_log` as the interna
 preserving the original query calls for the actual oracle responses.
 -/
 
-open oracle_comp oracle_spec
+open oracle_comp oracle_spec sim_oracle
 
 variables {α β γ : Type} {spec : oracle_spec}
 
 /-- Simulation oracle for logging the queries made during the computation,
 tracked via a `query_log`, whithout modifying the query calls themselves. -/
-def logging_oracle (spec : oracle_spec) : sim_oracle spec spec (query_log spec) :=
+@[inline, reducible] def logging_oracle (spec : oracle_spec) :
+  sim_oracle spec spec (query_log spec) :=
 ⟪query | query_log.log_query, ∅⟫
 
 notation `loggingₛₒ` := logging_oracle _
+
+lemma logging_oracle.def : logging_oracle spec = ⟪query | query_log.log_query, ∅⟫ := rfl
 
 instance logging_oracle.is_tracking : (logging_oracle spec).is_tracking :=
 tracking_oracle.is_tracking query query_log.log_query ∅
 
 namespace logging_oracle
 
--- TODO
+lemma apply_eq {i : spec.ι} (t : spec.domain i) (qc : spec.query_log) :
+  loggingₛₒ i (t, qc) = (λ u, (u, qc.log_query i t u)) <$> (query i t) := rfl
+
+lemma answer_query_eq : (logging_oracle spec).answer_query = query := rfl
+
+lemma update_state_eq : (logging_oracle spec).update_state = query_log.log_query := rfl
+
+section simulate'
+
+variables (oa : oracle_comp spec α) (s : spec.query_log)
+
+@[pairwise_dist_equiv] lemma simulate'_dist_equiv : simulate' loggingₛₒ oa s ≃ₚ oa :=
+is_tracking.simulate'_dist_equiv_self loggingₛₒ oa s (λ i t, dist_equiv.rfl)
+
+@[simp] lemma support_simulate' : (simulate' loggingₛₒ oa s).support = oa.support :=
+by pairwise_dist_equiv
+
+@[simp] lemma fin_support_simulate' : (simulate' loggingₛₒ oa s).fin_support = oa.fin_support :=
+by pairwise_dist_equiv
+
+@[simp] lemma eval_dist_simulate' : ⁅simulate' loggingₛₒ oa s⁆ = ⁅oa⁆ :=
+by pairwise_dist_equiv
+
+@[simp] lemma prob_output_simulate' (x : α) : ⁅= x | simulate' loggingₛₒ oa s⁆ = ⁅= x | oa⁆ :=
+by pairwise_dist_equiv
+
+@[simp] lemma prob_event_simulate' (e : set α) : ⁅e | simulate' loggingₛₒ oa s⁆ = ⁅e | oa⁆ :=
+by pairwise_dist_equiv
+
+end simulate'
 
 end logging_oracle
